set up function lemma for monomorphic functions

theories/iris/logrel/function.v
@@ -1,10 +1,13 @@
 From iris.proofmode Require Export base proofmode classes.
 
-From RichWasm Require Import syntax typing.
+From RichWasm Require Import syntax typing named_props.
 From RichWasm.compiler Require Import prelude module.
 Require Import RichWasm.iris.host.iris_host.
 Require Import RichWasm.iris.rules.iris_rules.
 From RichWasm.iris Require Import logrel memory util.
+From RichWasm.iris Require Import logrel.instr.typing.
+From RichWasm.iris Require Import logrel.logrel_properties.
+From RichWasm.iris Require Import language.cwp.
 
 Module W := RichWasm.wasm.datatypes.
 
@@ -20,24 +23,234 @@ Section function.
   Variable rti : rt_invariant Σ.
   Variable sr : store_runtime.
 
-  Theorem fundamental_function mr M wt wt' wtf mf mf' ϕ :
+  Lemma bind_inr {A B C} (mx : A + B) (f : B -> A + C) (y : C) :
+    mx ≫= f = inr y ↔ ∃ x : B, mx = inr x /\ f x = inr y.
+  Proof.
+    split.
+    - intros H. destruct mx; first inversion H. by exists b.
+    - by intros (x & -> & Hfx).
+  Qed.
+
+  Lemma try_opt_inr {E A} (err : E) c (a : A) :
+    util.try_option err c = inr a →
+    c = Some a.
+  Proof.
+    destruct c; cbn; intros Heq; by inversion Heq.
+  Qed.
+
+  Lemma insert_type_inst_get mr M wt tf wt' tid wtf inst :
+    ⌜insert_type wt tf = (wt', tid)⌝ -∗
+    instance_interp rti sr mr M (wt ++ option_list wt' ++ wtf) inst -∗
+    ⌜inst_types inst !! tid = Some tf⌝.
+  Proof.
+  Admitted.
+
+  Definition atom_zero (ι : atomic_rep) : atom :=
+    match ι with
+    | PtrR => PtrA (PtrInt 0%N)
+    | I32R => I32A (Wasm_int.int_zero i32m)
+    | I64R => I64A (Wasm_int.int_zero i64m)
+    | F32R => F32A (Wasm_float.float_zero f32m)
+    | F64R => F64A (Wasm_float.float_zero f64m)
+    end.
+
+  Lemma big_sepL2_concat_inv_l {X Y} {P : X → Y → iProp Σ} xss ys :
+    ([∗ list] x; y ∈ concat xss; ys, P x y) -∗
+    ∃ yss, ⌜ys = concat yss⌝ ∗ ([∗ list] xs; ys ∈ xss; yss, [∗ list] x; y ∈ xs; ys, P x y).
+  Proof.
+    revert ys.
+    induction xss; iIntros (ys) "Hall".
+    - iPoseProof (big_sepL2_nil_inv_l with "Hall") as "->".
+      iExists [].
+      by rewrite big_sepL2_nil.
+    - cbn [concat].
+      iPoseProof (big_sepL2_app_inv_l with "Hall") as "(%ys1 & %ys2 & -> & Hys1 & Hys2)".
+      iPoseProof (IHxss with "Hys2") as "(%yss & -> & Hyss)".
+      iExists (ys1 :: yss).
+      by iFrame.
+  Qed.
+
+  Theorem fund_function_mono τs1 τs2 M wt wt' wtf mf mf' :
+    has_function_type M mf (MonoFunT τs1 τs2) →
+    compile_function wt mf = inr (wt', mf') →
+    ⊢ has_func_type_sem rti sr module.mr M (wt ++ wt' ++ wtf) mf' (MonoFunT τs1 τs2).
+  Proof.
+    iIntros (Hϕ Hcf ?? Htf) "#Hinst".
+
+    (* Open up the typing judgment *)
+    inversion Hϕ.
+    subst M0 mf0 ϕ ϕ0.
+    set (fft := flatten_function_type mf.(mf_type)) in *.
+
+    rename H0 into Hηss_L.
+    rename H1 into Hρs_P.
+    rename H2 into Hηss_P.
+    rename H6 into Hψ.
+    rename H3 into HL'.
+    rename H into Hty.
+    destruct tf as [ts1 ts2].
+
+    (* Open up the compiler *)
+    apply bind_inr in Hcf.
+    destruct Hcf as (ft & Hft & Hcf).
+    destruct (insert_type wt ft) as [wt'' tid] eqn:Htid.
+    apply bind_inr in Hcf.
+    destruct Hcf as (fe & Hfe & Hcf).
+    apply bind_inr in Hcf.
+    destruct Hcf as (res & Hcg & Hcf).
+    destruct res as [[[[] wt_es] wl_es] es].
+    apply bind_inr in Hcf.
+    destruct Hcf as (ιs & Hevrep & Hcf).
+    inversion Hcf; subst; clear Hcf.
+    cbn.
+
+    rewrite Hty in Hft.
+    apply try_opt_inr in Hft.
+    apply bind_Some in Hft.
+    destruct Hft as (ts1' & Hts1' & Hft).
+    apply bind_Some in Hft.
+    destruct Hft as (ts2' & Hts2' & Hft).
+    inversion Hft; subst ft.
+    cbn in Htf.
+    rewrite -app_assoc.
+    iPoseProof (insert_type_inst_get with "[//] Hinst") as "%Hget".
+    rewrite Hget in Htf; inversion Htf; subst ts1' ts2'.
+
+    (* Show the function env matches what F says *)
+    assert (fe_of_context F = fe).
+    {
+      revert Hfe; intros Hfe.
+      unfold fe_of_context; cbn.
+      apply try_opt_inr in Hfe.
+      apply bind_Some in Hfe.
+      destruct Hfe as (ρs_fe & Hρs & Hfe).
+      apply bind_Some in Hfe.
+      destruct Hfe as (ηss_P' & HηP' & Hfe).
+      apply bind_Some in Hfe.
+      destruct Hfe as (ηss_L' & HηL' & Hfe).
+      inversion Hfe.
+      unfold fft; cbn.
+      f_equal.
+      cbn in HηP', HηL'.
+      assert (ρs_fe = ρs_P).
+      { admit. }
+      subst ρs_fe.
+      rewrite Hηss_P in HηP'.
+      rewrite Hηss_L in HηL'.
+      congruence.
+    }
+    subst fe.
+
+    unfold ψ in Hψ; clear ψ.
+    unfold fft in Hψ.
+    rewrite Hty in Hψ.
+    cbn in Hψ.
+
+    (* Obtain the semantic typing for the body of the fn *)
+    pose proof Hψ as Hsem.
+    eapply (fundamental_typing rti sr) in Hsem; last apply Hcg.
+    instantiate (2 := wtf) in Hsem.
+    clear_nils.
+
+    (* now deal with closure_interp' *)
+    rewrite closure_interp_eq.
+    unfold closure_interp'.
+    rewrite Hty.
+    unfold mono_closure_interp.
+    cbn -[atom_interp translate_types].
+    assert (translate_types (Σ:=Σ) senv_empty τs1 = prelude.translate_types [] τs1) as Htrans1.
+    { admit. }
+    assert (translate_types (Σ:=Σ) senv_empty τs2 = prelude.translate_types [] τs2) as Htrans2.
+    { admit. }
+    iSplitR; last iSplitR.
+    (* For both of these admits, we have to relate prelude.translate_types and
+       logrel.translate_types. *)
+    { by rewrite Htrans1 Hts1'. }
+    { by rewrite Htrans2 Hts2'. }
+    iIntros "!> !>".
+    iIntros (vs1 os1 θ) "Hats Hoss Htok Hmask Hf Hr".
+    unfold have_instr_type_sem in Hsem.
+    set (fr := {| W.f_locs := vs1 ++ n_zeros (flat_map (map translate_arep) ιs ++ wl_es);
+                 W.f_inst := inst |}).
+    iPoseProof (Hsem $! senv_empty fr _ _ [] with "[] [] Hinst") as "Hsem"; clear Hsem.
+    { iPureIntro.
+      unfold sem_env_interp, F, K, fft, kc_of_fft; cbn.
+      rewrite Hty; cbn.
+      split.
+      - done.
+      - constructor.
+    }
+    {
+      by instantiate (1 := []).
+    }
+    clear_nils.
+    iApply (cwp_wand with "[-]").
+    { iApply ("Hsem" with "[] [] [] [] [Hoss Hats] Htok Hmask Hf Hr"); iClear "Hsem".
+      - unfold labels_interp.
+        simpl fc_labels.
+        unfold fft.
+        rewrite Hty.
+        iApply big_sepL2_singleton.
+        iSplitR.
+        { by rewrite Htrans2 Hts2'. }
+        iModIntro.
+        iIntros (fr' vs' os' θ') "%Hrel Hfr Htok Hinv Hats Hvs".
+        iFrame.
+      - unfold return_interp.
+        unfold F; cbn [fc_return].
+        unfold fft.
+        rewrite Hty.
+        iSplitR.
+        { by rewrite Htrans2 Hts2'. }
+        iModIntro.
+        iIntros (vs' os' θ') "Hats Hvs Htok Hinv".
+        iFrame.
+      - by iApply big_sepL2_nil.
+      - iExists [].
+        iSplit; first done.
+        by rewrite big_sepL2_nil.
+      - unfold frame_interp. cbn -[atom_interp].
+        iDestruct "Hoss" as "(%oss & -> & Hoss)".
+        setoid_rewrite big_sepL2_fmap_l.
+        unfold L, fft.
+        rewrite Hty.
+        cbn [flatten_function_type fft_in].
+        iPoseProof (big_sepL2_concat_inv_l with "Hats") as "(%vss & -> & Hats)".
+        iExists (oss ++ map (map atom_zero) ιs).
+        iExists (vss ++ (map (n_zeros ∘ map translate_arep) ιs)).
+        iExists (n_zeros wl_es).
+        iFrame.
+        repeat iSplitR; try iPureIntro.
+        + unfold n_zeros; change @seq.map with @map.
+          rewrite map_app concat_app -app_assoc.
+          f_equal.
+          f_equal.
+          rewrite flat_map_concat_map.
+          rewrite concat_map.
+          rewrite map_map.
+          done.
+        + admit.
+        + admit.
+        + repeat setoid_rewrite big_sepL2_fmap_l.
+          repeat setoid_rewrite big_sepL2_fmap_r.
+          iApply big_sepL_sepL2_diag.
+          admit.
+        + repeat setoid_rewrite big_sepL2_fmap_l.
+          repeat setoid_rewrite big_sepL2_fmap_r.
+          admit.
+    }
+    {
+      iIntros (f v)
+       "(%Hfrel & Hfr & (%os_ret & Hos_ret & Hats_ret) & (%θ' & Htok) & Hinv)".
+      by iFrame.
+    }
+  Admitted.
+
+  Theorem fundamental_function ϕ : ∀ mr M wt wt' wtf mf mf',
     has_function_type M mf ϕ ->
     compile_function wt mf = inr (wt', mf') ->
     ⊢ has_func_type_sem rti sr mr M (wt ++ wt' ++ wtf) mf' ϕ.
   Proof.
-    iIntros (Hϕ Hcf ?? Htf) "#Hinst".
-    inversion Hϕ.
-    subst M0 mf0 ϕ ϕ0 ϕ1.
-    set (ϕ := mf.(mf_type)) in *.
-    set (fft := flatten_function_type ϕ) in *.
-    rename H into Hηss_L.
-    rename H0 into Hρs_P.
-    rename H1 into Hηss_P.
-    rename H3 into Hψ.
-    rename H2 into HL'.
-    destruct tf as [ts1 ts2].
-    rewrite closure_interp_eq.
-
     (* TODO: By induction on ϕ, build up an se such that sem_env_interp F se.
              Then use the fundamental theorem for instruction typing to show that the body of the
              function is well-behaved. *)
